StrataTest/Languages/Core/Examples/ProcedureCall.lean
@@ -70,18 +70,18 @@ VCs:
 Label: new_g_value
 Property: assert
 Assumptions:
-counter_ge_zero: $__counter2 >= 0
-a_positive: $__a1 > 0
+counter_ge_zero: $__counter1 >= 0
+a_positive: $__a2 > 0
 Obligation:
 true
 
 Label: old_g_property
 Property: assert
 Assumptions:
-counter_ge_zero: $__counter2 >= 0
-a_positive: $__a1 > 0
+counter_ge_zero: $__counter1 >= 0
+a_positive: $__a2 > 0
 Obligation:
-$__counter2 + $__a1 - $__a1 == $__counter2
+$__counter1 + $__a2 - $__a2 == $__counter1
 
 Label: (Origin_Inc_Requires)counter_ge_zero
 Property: assert
@@ -101,17 +101,17 @@ Label: (Origin_Inc_Requires)counter_ge_zero
 Property: assert
 Assumptions:
 counter_ge_zero: $__counter5 >= 0
-(Origin_Inc_Ensures)new_g_value: $__counter9 == $__counter5 + 8
-(Origin_Inc_Ensures)old_g_property: $__b8 - 8 == $__counter5
+(Origin_Inc_Ensures)new_g_value: $__counter8 == $__counter5 + 8
+(Origin_Inc_Ensures)old_g_property: $__b9 - 8 == $__counter5
 Obligation:
-$__counter9 >= 0
+$__counter8 >= 0
 
 Label: (Origin_Inc_Requires)a_positive
 Property: assert
 Assumptions:
 counter_ge_zero: $__counter5 >= 0
-(Origin_Inc_Ensures)new_g_value: $__counter9 == $__counter5 + 8
-(Origin_Inc_Ensures)old_g_property: $__b8 - 8 == $__counter5
+(Origin_Inc_Ensures)new_g_value: $__counter8 == $__counter5 + 8
+(Origin_Inc_Ensures)old_g_property: $__b9 - 8 == $__counter5
 Obligation:
 true
 
@@ -119,12 +119,12 @@ Label: return_value_lemma
 Property: assert
 Assumptions:
 counter_ge_zero: $__counter5 >= 0
-(Origin_Inc_Ensures)new_g_value: $__counter9 == $__counter5 + 8
-(Origin_Inc_Ensures)old_g_property: $__b8 - 8 == $__counter5
-(Origin_Inc_Ensures)new_g_value: $__counter11 == $__counter9 + 8
-(Origin_Inc_Ensures)old_g_property: $__b10 - 8 == $__counter9
+(Origin_Inc_Ensures)new_g_value: $__counter8 == $__counter5 + 8
+(Origin_Inc_Ensures)old_g_property: $__b9 - 8 == $__counter5
+(Origin_Inc_Ensures)new_g_value: $__counter10 == $__counter8 + 8
+(Origin_Inc_Ensures)old_g_property: $__b11 - 8 == $__counter8
 Obligation:
-$__b10 == $__counter5 + 16
+$__b11 == $__counter5 + 16
 
 Label: assert_0
 Property: assert
