StrataTest/Transform/CallElim.lean
@@ -62,14 +62,14 @@ procedure h() returns () spec {
   modifies j;
 } {
   var b : bool;
-  var tmp_arg_0 : bool := k;
-  var tmp_arg_1 : bool := j;
-  var tmp_b_2 : bool := b;
-  var tmp_j_3 : bool := j;
-  assert [callElimAssert_f_requires_0_4]: (i == (!tmp_arg_0));
-  havoc b;
+  var tmp_arg_0 : bool := j;
+  var tmp_arg_1 : bool := k;
+  var tmp_j_2 : bool := j;
+  var tmp_b_3 : bool := b;
+  assert [callElimAssert_f_requires_0_4]: (i == (!tmp_arg_1));
   havoc j;
-  assume [callElimAssume_f_ensures_1_5]: (b == tmp_arg_0);
+  havoc b;
+  assume [callElimAssume_f_ensures_1_5]: (b == tmp_arg_1);
   assume [callElimAssume_f_ensures_2_6]: (b == j);
 };
 #end
@@ -114,15 +114,15 @@ procedure h() returns () spec {
   modifies j;
 } {
   var b : bool;
-  var tmp_arg_0 : bool := k;
-  var tmp_arg_1 : bool := l;
-  var tmp_arg_2 : bool := j;
-  var tmp_b_3 : bool := b;
-  var tmp_j_4 : bool := j;
+  var tmp_arg_0 : bool := j;
+  var tmp_arg_1 : bool := k;
+  var tmp_arg_2 : bool := l;
+  var tmp_j_3 : bool := j;
+  var tmp_b_4 : bool := b;
   var old_j_5 : bool := j;
-  assert [callElimAssert_f_requires_0_6]: i == !tmp_arg_0;
-  havoc b;
+  assert [callElimAssert_f_requires_0_6]: i == !tmp_arg_1;
   havoc j;
+  havoc b;
   assume [callElimAssume_f_ensures_1_7]: b == (k && old_j_5);
   assume [callElimAssume_f_ensures_2_8]: b == old_j_5;
 };
@@ -168,15 +168,15 @@ procedure h() returns () spec {
   modifies j;
 } {
   var b : bool;
-  var tmp_arg_0 : bool := k && i || j;
-  var tmp_arg_1 : bool := l;
-  var tmp_arg_2 : bool := j;
-  var tmp_b_3 : bool := b;
-  var tmp_j_4 : bool := j;
+  var tmp_arg_0 : bool := j;
+  var tmp_arg_1 : bool := k && i || j;
+  var tmp_arg_2 : bool := l;
+  var tmp_j_3 : bool := j;
+  var tmp_b_4 : bool := b;
   var old_j_5 : bool := j;
-  assert [callElimAssert_f_requires_0_6]: i == !tmp_arg_0;
-  havoc b;
+  assert [callElimAssert_f_requires_0_6]: i == !tmp_arg_1;
   havoc j;
+  havoc b;
   assume [callElimAssume_f_ensures_1_7]: b == (k && old_j_5);
   assume [callElimAssume_f_ensures_2_8]: b == old_j_5;
 };
@@ -219,14 +219,14 @@ procedure h() returns () spec {
   modifies j;
 } {
   var b : bool;
-  var tmp_arg_0 : bool := k;
-  var tmp_arg_1 : bool := j;
-  var tmp_b_2 : bool := b;
-  var tmp_j_3 : bool := j;
-  assert [callElimAssert_f_requires_1_4]: (tmp_arg_0 == tmp_arg_1);
-  havoc b;
+  var tmp_arg_0 : bool := j;
+  var tmp_arg_1 : bool := k;
+  var tmp_j_2 : bool := j;
+  var tmp_b_3 : bool := b;
+  assert [callElimAssert_f_requires_1_4]: (tmp_arg_1 == tmp_arg_0);
   havoc j;
-  assume [callElimAssume_f_ensures_2_5]: (b == tmp_arg_0);
+  havoc b;
+  assume [callElimAssume_f_ensures_2_5]: (b == tmp_arg_1);
 };
 #end
 
